remove global lock, atomic accesses; harmonize return types; separate handle

steel/Zeta.Steel.SafeMain.fst
@@ -1,263 +1,36 @@
 module Zeta.Steel.SafeMain
+open Zeta.Steel.SafeMain.Handle
 
 module Lock = Steel.ST.SpinLock
 module R = Steel.ST.Reference
 
 open Steel.ST.GenElim
 
-// TODO: use FStarLang/FStar#2349 to nest structs and take pointers to fields. However, we need support for atomic accesses for such references, at least for the top-level cases (so far we don't need atomic field accesses here yet)
-
-[@@__reduce__]
-let thread_lock_vprop
-  (tl_state: M.top_level_state)
-  (tid: AT.tid)
-: Tot vprop
-= exists_ (fun (entries: AEH.log) -> M.log_of_tid tl_state tid entries)
-
-let thread_lock_t
-  (tl_state: M.top_level_state)
-: Tot Type
-= (tid: Ghost.erased AT.tid & Lock.lock (thread_lock_vprop tl_state tid))
-
-let thread_state_prop
-  (#tl_state: M.top_level_state)
-  (a: Seq.seq (thread_lock_t tl_state))
-: Tot prop
-= forall (i: nat { i < Seq.length a }) . {:pattern (Seq.index a i)} U16.v (dfst (Seq.index a i)) == i
-
-noeq
-type state_t = {
-  state: R.ref M.top_level_state;
-  tl_state: Ghost.erased M.top_level_state;
-  thread_locks: A.array (thread_lock_t tl_state);
-  tl_thread_locks: Ghost.erased (Seq.seq (thread_lock_t tl_state));
-  tl_frozen_logs: Ghost.erased M.tid_log_map;
-  tl_prf: squash (thread_state_prop tl_thread_locks /\ Seq.length tl_thread_locks == U32.v AT.n_threads);
-}
-
-[@@__reduce__]
-let state_ptr_inv_null
-  (p: perm)
-: Tot vprop
-= pure (p == full_perm)
-
-[@@__reduce__]
-let handle_pts_to_body0
-  (r2: state_t)
-: Tot vprop
-= exists_ (fun p3 -> exists_ (fun p4 ->
-    R.pts_to r2.state p3 r2.tl_state `star`
-    A.pts_to r2.thread_locks p4 r2.tl_thread_locks `star`
-    M.core_inv r2.tl_state `star`
-    M.frozen_logs r2.tl_state r2.tl_frozen_logs
-  ))
-
-let handle_pts_to_body
-  (r2: state_t)
-: Tot vprop
-= handle_pts_to_body0 r2
-
-[@@__reduce__]
-let state_ptr_inv_not_null_body
-  (state: R.ref state_t)
-  (st: state_t)
-: Tot vprop
-= exists_ (fun p1 ->
-    R.pts_to state p1 st `star`
-    handle_pts_to_body st
-  )
-
-[@@__reduce__]
-let state_ptr_inv_not_null
-  (state: R.ref state_t)
-: Tot vprop
-= exists_ (fun st ->
-    state_ptr_inv_not_null_body state st
-  )
-
-let state_ptr_inv_if
-  (state: R.ref state_t)
-  (p: perm)
-: Tot vprop
-= if R.is_null state
-  then state_ptr_inv_null p
-  else state_ptr_inv_not_null state
-
-[@@__reduce__]
-let state_ptr_inv0
-  (state_ptr: R.ref (R.ref state_t))
-: Tot vprop
-= exists_ (fun p -> exists_ (fun state ->
-    R.pts_to state_ptr (half_perm p) state `star`
-    state_ptr_inv_if state p
-  ))
-
-let state_ptr_inv
-  (state_ptr: R.ref (R.ref state_t))
-: Tot vprop
-= state_ptr_inv0 state_ptr
-
-let state_ptr_lock_prop
-  (state: R.ref state_t)
-  (p: perm)
-: Tot prop
-= R.is_null state == true ==> p == full_perm
-
-[@@__reduce__]
-let state_ptr_lock0
-  (state_ptr: R.ref (R.ref state_t))
-: Tot vprop
-= exists_ (fun p -> exists_ (fun state ->
-    R.pts_to state_ptr (half_perm p) state `star`
-    pure (state_ptr_lock_prop state p)
-  ))
-
-let state_ptr_lock
-  (state_ptr: R.ref (R.ref state_t))
-: Tot vprop
-= state_ptr_lock0 state_ptr
-
-noeq
-type handle_t = {
-  state_ptr: R.ref (R.ref state_t);
-  _inv: inv (state_ptr_inv state_ptr);
-  _lock: Lock.lock (state_ptr_lock state_ptr);
-}
-
-let create_handle () : STT handle_t emp (fun _ -> emp) =
-  let state_ptr : R.ref (R.ref state_t) = R.alloc R.null in
-  R.share state_ptr;
-  (* invariant *)
-  rewrite (state_ptr_inv_null full_perm) (state_ptr_inv_if R.null full_perm);
-  rewrite (state_ptr_inv0 state_ptr) (state_ptr_inv state_ptr);
-  let _inv = new_invariant (state_ptr_inv state_ptr) in
-  (* lock *)
-  rewrite (state_ptr_lock0 state_ptr) (state_ptr_lock state_ptr);
-  let _lock = Lock.new_lock (state_ptr_lock state_ptr) in
-  (* summary *)
-  return ({
-    state_ptr = state_ptr;
-    _inv = _inv;
-    _lock = _lock;
-  })
-
-let handle = create_handle () 
-
-[@@__reduce__]
-let handle_pts_to_aux0
-  (r2: state_t)
-: Tot vprop
-= exists_ (fun p1 -> exists_ (fun r1 ->
-    R.pts_to handle.state_ptr p1 r1 `star`
-    state_ptr_inv_not_null_body r1 r2
-  ))
-
-let handle_pts_to_aux
-  (r2: state_t)
-: Tot vprop
-= handle_pts_to_aux0 r2
-
 [@@__reduce__]
 let handle_pts_to0
   (ts: M.top_level_state)
 : Tot vprop
-= exists_ (fun r2 ->
-    handle_pts_to_aux r2 `star`
-    pure (ts == Ghost.reveal r2.tl_state)
-  )
+= handle_pts_to_body handle.state `star`
+  pure (ts == Ghost.reveal handle.state.tl_state)
 
 let handle_pts_to
   (ts: M.top_level_state)
 : Tot vprop
 = handle_pts_to0 ts
-
-let gather_body
-  (#opened: _)
-  (r2: state_t)
-: STGhostT unit opened
-    (handle_pts_to_body r2 `star` handle_pts_to_body r2)
-    (fun _ -> handle_pts_to_body r2)
-= rewrite (handle_pts_to_body r2) (handle_pts_to_body0 r2);
-  let _ = gen_elim () in
-  let ps = vpattern_replace (fun ps -> R.pts_to r2.state ps _) in
-  let pa = vpattern_replace (fun pa -> A.pts_to r2.thread_locks pa _) in
-  rewrite (handle_pts_to_body r2) (handle_pts_to_body0 r2);
-  let _ = gen_elim () in
-  A.gather r2.thread_locks pa _;
-  R.gather ps r2.state;
-  M.core_inv_gather _;
-  M.frozen_logs_gather _ _;
-  rewrite (handle_pts_to_body0 r2) (handle_pts_to_body r2)
-
-let gather_aux
-  (#opened: _)
-  (ts1: state_t)
-  (ts2: state_t)
-: STGhost unit opened
-    (handle_pts_to_aux ts1 `star` handle_pts_to_aux ts2)
-    (fun _ -> handle_pts_to_aux ts1)
-    True
-    (fun _ -> ts1 == ts2)
-= rewrite (handle_pts_to_aux ts1) (handle_pts_to_aux0 ts1);
-  let _ = gen_elim () in
-  let r1 = vpattern_replace (fun r1 -> R.pts_to handle.state_ptr _ r1 `star` R.pts_to r1 _ _) in
-  rewrite (handle_pts_to_aux ts2) (handle_pts_to_aux0 ts2);
-  let _ = gen_elim () in
-  let r2 = vpattern_replace (fun r2 -> R.pts_to handle.state_ptr _ r1 `star` R.pts_to handle.state_ptr _ r2 `star` R.pts_to r2 _ _) in
-  R.gather _ #r1 handle.state_ptr;
-  vpattern_rewrite #_ #_ #r2 (fun r2 -> R.pts_to r2 _ _) r1;
-  R.gather _ #ts1 r1;
-  rewrite (handle_pts_to_body ts2) (handle_pts_to_body ts1);
-  gather_body ts1;
-  rewrite (handle_pts_to_aux0 ts1) (handle_pts_to_aux ts1)
   
 let gather ts ts' =
   rewrite (handle_pts_to ts) (handle_pts_to0 ts);
   let _ = gen_elim () in
-  let ts1 = vpattern_replace handle_pts_to_aux in
   rewrite (handle_pts_to ts') (handle_pts_to0 ts');
   let _ = gen_elim () in
-  gather_aux ts1 _;
+  gather_body _;
   rewrite (handle_pts_to0 ts) (handle_pts_to ts)
-
-let share_body
-  (#opened: _)
-  (r2: state_t)
-: STGhostT unit opened
-    (handle_pts_to_body r2)
-    (fun _ -> handle_pts_to_body r2 `star` handle_pts_to_body r2)
-= rewrite (handle_pts_to_body r2) (handle_pts_to_body0 r2);
-  let _ = gen_elim () in
-  let pa = vpattern_replace (fun pa -> A.pts_to r2.thread_locks pa _) in
-  A.share r2.thread_locks pa (half_perm pa) (half_perm pa);
-  R.share r2.state;
-  M.core_inv_share _;
-  M.frozen_logs_share _ _;
-  rewrite (handle_pts_to_body0 r2) (handle_pts_to_body r2);
-  noop ();
-  rewrite (handle_pts_to_body0 r2) (handle_pts_to_body r2)
-
-let share_aux
-  (#opened: _)
-  (r2: state_t)
-: STGhostT unit opened
-    (handle_pts_to_aux r2)
-    (fun _ -> handle_pts_to_aux r2 `star` handle_pts_to_aux r2)
-= rewrite (handle_pts_to_aux r2) (handle_pts_to_aux0 r2);
-  let _ = gen_elim () in
-  let r1 = vpattern_replace (fun r1 -> R.pts_to handle.state_ptr _ r1 `star` R.pts_to r1 _ _) in
-  R.share handle.state_ptr;
-  R.share r1;
-  share_body r2;
-  rewrite (handle_pts_to_aux0 r2) (handle_pts_to_aux r2);
-  noop ();
-  rewrite (handle_pts_to_aux0 r2) (handle_pts_to_aux r2)
 
 let share
   ts
 = rewrite (handle_pts_to ts) (handle_pts_to0 ts);
   let _ = gen_elim () in
-  share_aux _;
+  share_body _;
   rewrite (handle_pts_to0 ts) (handle_pts_to ts);
   noop ();
   rewrite (handle_pts_to0 ts) (handle_pts_to ts)
@@ -274,312 +47,24 @@ let with_invariant_g (#a:Type)
   : STGhostT a opened_invariants fp fp'
 = with_invariant_g i f
 
-assume
-val atomic_read_ref
-  (#t: Type)
-  (#opened:_)
-  (#p:perm)
-  (#v:Ghost.erased t)
-  (r:R.ref t)
-  : STAtomic t opened
-      (R.pts_to r p v)
-      (fun x -> R.pts_to r p v)
-      (requires True)
-      (ensures fun x -> x == Ghost.reveal v)
-
-assume
-val atomic_write_ref
-  (#t: Type)
-  (#opened:_)
-  (#v:Ghost.erased t)
-  (r:R.ref t)
-  (x:t)
-  : STAtomicT unit opened
-      (R.pts_to r full_perm v)
-      (fun _ -> R.pts_to r full_perm x)
-
-let handle_is_null_post (b: bool) : vprop =
-  if b
-  then emp
-  else exists_ handle_pts_to_aux
-
-inline_for_extraction
-let with_invariant (#a:Type)
-                   (#fp:vprop)
-                   (#fp':a -> vprop)
-                   (#opened_invariants:inames)
-                   (#p:vprop)
-                   (i:inv p{not (mem_inv opened_invariants i)})
-                   (f:unit -> STAtomicT a (add_inv opened_invariants i)
-                                          (p `star` fp)
-                                          (fun x -> p `star` fp' x))
-  : STAtomicT a opened_invariants fp fp'
-= with_invariant i f
-
-let handle_is_null
+let handle_pts_to_body_intro
   (#opened: _)
   ()
-: STAtomic bool opened
+: STGhost unit opened
     emp
-    (fun b -> handle_is_null_post b)
+    (fun _ -> handle_pts_to_body handle.state)
     (not (mem_inv opened handle._inv))
     (fun _ -> True)
-= noop (); // for pure
-  with_invariant
-    #bool
+= with_invariant_g
+    #unit
     #emp
-    #(fun b -> handle_is_null_post b)
+    #(fun _ -> handle_pts_to_body handle.state)
     #_
-    #(state_ptr_inv handle.state_ptr)
+    #(handle_pts_to_body handle.state)
     handle._inv
     (fun _ ->
-      rewrite
-        (state_ptr_inv handle.state_ptr)
-        (state_ptr_inv0 handle.state_ptr);
-      let _ = gen_elim () in
-      let state = atomic_read_ref handle.state_ptr in
-      if R.is_null state
-      then begin
-        noop ();
-        rewrite
-          (state_ptr_inv0 handle.state_ptr)
-          (state_ptr_inv handle.state_ptr);
-        rewrite
-          emp
-          (handle_is_null_post true);
-        return true
-      end else begin
-        let p = vpattern_replace (fun p -> R.pts_to handle.state_ptr (half_perm p) _ `star` state_ptr_inv_if _ p) in
-        let state = vpattern_replace_erased (fun state -> R.pts_to handle.state_ptr _ state `star` state_ptr_inv_if state _) in
-        rewrite
-          (state_ptr_inv_if _ _)
-          (state_ptr_inv_not_null state);
-        let _ = gen_elim () in
-        R.share handle.state_ptr;
-        let r2 = vpattern_replace_erased (fun r2 -> R.pts_to state _ r2 `star` handle_pts_to_body r2) in
-        share_body _;
-        R.share state;
-        (* invariant *)
-        rewrite
-          (state_ptr_inv_not_null state)
-          (state_ptr_inv_if state (half_perm p));
-        rewrite
-          (state_ptr_inv0 handle.state_ptr)
-          (state_ptr_inv handle.state_ptr);
-        (* handle_pts_to *)
-        rewrite
-          (handle_pts_to_aux0 r2)
-          (handle_pts_to_aux0 r2);
-        rewrite 
-          (exists_ handle_pts_to_aux)
-          (handle_is_null_post false);
-        return false
-      end
+      share_body _
     )
-
-let seq_lemma_index_upd
-  (#a:Type)
-  (s:Seq.seq a)
-  (n:nat{n < Seq.length s})
-  (v:a)
-: Lemma
-  (requires True)
-  (ensures (forall i . Seq.index (Seq.upd s n v) i == (if i = n then v else Seq.index s i)))
-= ()
-
-// TODO: replace this function with a Steel.ST.Loops.while_loop
-let rec init_thread_locks_loop
-  (tl_state: Ghost.erased M.top_level_state)
-  (tl_logs: Ghost.erased M.tid_log_map)
-  (tl: A.array (thread_lock_t tl_state))
-  (a0: Ghost.erased (Seq.seq (thread_lock_t tl_state)))
-  (tid: U16.t)
-: ST unit
-    (M.all_logs tl_state tl_logs `star` A.pts_to tl full_perm a0)
-    (fun _ ->
-      exists_ (fun l' -> M.frozen_logs tl_state l') `star`
-      exists_ (fun a ->
-      A.pts_to tl full_perm a `star`
-      pure (thread_state_prop a /\ Seq.length a == U32.v AT.n_threads)
-    ))
-    (A.length tl == U32.v AT.n_threads /\
-      Seq.length (Ghost.reveal a0) == U32.v AT.n_threads /\
-      U16.v tid <= U32.v AT.n_threads /\
-      (forall (i: nat) . i < U16.v tid ==> U16.v (Ghost.reveal (dfst (Seq.index (Ghost.reveal a0) i))) == i) /\
-      (forall (i: AT.tid) . U16.v i >= U16.v tid ==> Some? (Map.sel tl_logs i))
-    )
-    (fun _ -> True)
-= let tid32 = FStar.Int.Cast.uint16_to_uint32 tid in
-  if tid32 = AT.n_threads
-  then begin
-    M.freeze_all_logs _ _;
-    return ()
-  end
-  else begin
-    M.all_logs_log_of_tid _ _ tid ();
-    let l = Lock.new_lock (thread_lock_vprop tl_state tid) in
-    let t : thread_lock_t tl_state = (| Ghost.hide tid, l |) in
-    A.write tl tid32 t;
-    Seq.lemma_len_upd (U32.v tid32) t a0;
-    seq_lemma_index_upd a0 (U32.v tid32) t;
-    init_thread_locks_loop tl_state _ tl _ (tid `U16.add` 1us)
-  end
-
-let init_thread_locks
-  (tl_state: Ghost.erased M.top_level_state)
-  (tl_logs: Ghost.erased M.tid_log_map)
-: ST (A.array (thread_lock_t tl_state))
-    (M.all_logs tl_state tl_logs)
-    (fun tl ->
-      exists_ (fun l' -> M.frozen_logs tl_state l') `star`
-      exists_ (fun a ->
-        A.pts_to tl full_perm a `star`
-        pure (thread_state_prop a /\ Seq.length a == U32.v AT.n_threads)
-    ))
-    (forall (i: AT.tid) . Some? (Map.sel tl_logs i))
-    (fun _ -> True)
-= M.all_logs_log_of_tid _ _ 0us ();
-  let l0 = Lock.new_lock (thread_lock_vprop tl_state 0us) in
-  let tl0: thread_lock_t tl_state = (| Ghost.hide 0us, l0 |) in
-  let tl = A.alloc tl0 AT.n_threads in
-  Seq.lemma_create_len (U32.v AT.n_threads) tl0;
-  Seq.lemma_index_create (U32.v AT.n_threads) tl0 0;
-  init_thread_locks_loop _ _ tl _ 1us;
-  return tl
-
-#push-options "--z3rlimit 32"
-#restart-solver
-
-let init ()
-= Lock.acquire handle._lock;
-  rewrite (state_ptr_lock handle.state_ptr) (state_ptr_lock0 handle.state_ptr);
-  let _ = gen_elim () in
-  let state = R.read handle.state_ptr in
-  if R.is_null state
-  then begin
-    let r2_state = M.init () in
-    let ts = elim_exists () in
-    let tl = init_thread_locks ts _ in
-    let _ = gen_elim () in
-    let tl_f = vpattern_replace_erased (M.frozen_logs ts) in
-    let tl_a = vpattern_replace_erased (A.pts_to tl _) in
-    [@@inline_let]
-    let r2 = ({
-      state = r2_state;
-      tl_state = ts;
-      thread_locks = tl;
-      tl_thread_locks = tl_a;
-      tl_frozen_logs = tl_f;
-      tl_prf = ();
-    })
-    in
-    let state' = R.alloc r2 in
-    R.pts_to_not_null state';
-    rewrite (R.pts_to r2_state full_perm _) (R.pts_to r2.state full_perm r2.tl_state);
-    rewrite (A.pts_to _ _ _) (A.pts_to r2.thread_locks full_perm r2.tl_thread_locks);
-    rewrite (M.frozen_logs _ _) (M.frozen_logs r2.tl_state r2.tl_frozen_logs);
-    rewrite (R.pts_to handle.state_ptr _ _) (R.pts_to handle.state_ptr (half_perm full_perm) state);
-    vpattern_rewrite M.core_inv (Ghost.reveal r2.tl_state);
-    rewrite (handle_pts_to_body0 r2) (handle_pts_to_body r2);
-    share_body _;
-    R.share state';
-    with_invariant
-      #unit
-      #(R.pts_to handle.state_ptr (half_perm full_perm) state `star` R.pts_to state' (half_perm full_perm) r2 `star` handle_pts_to_body r2)
-      #(fun _ -> R.pts_to handle.state_ptr (half_perm full_perm) state')
-      #_
-      #(state_ptr_inv handle.state_ptr)
-      (handle._inv)
-      (fun _ ->
-        rewrite (state_ptr_inv handle.state_ptr) (state_ptr_inv0 handle.state_ptr);
-        let _ = gen_elim () in
-        R.gather (half_perm full_perm) handle.state_ptr;
-        let p = vpattern_replace (state_ptr_inv_if _) in
-        rewrite
-          (state_ptr_inv_if _ _)
-          (state_ptr_inv_null p);
-        let _ = gen_elim () in
-        vpattern_rewrite (fun p -> R.pts_to handle.state_ptr p _) full_perm;
-        atomic_write_ref handle.state_ptr state';
-        R.share handle.state_ptr;
-        rewrite
-          (state_ptr_inv_not_null state')
-          (state_ptr_inv_if state' full_perm);
-        rewrite
-          (state_ptr_inv0 handle.state_ptr)
-          (state_ptr_inv handle.state_ptr);
-        noop ()
-      );
-    R.share handle.state_ptr;
-    rewrite (state_ptr_lock0 handle.state_ptr) (state_ptr_lock handle.state_ptr);
-    Lock.release handle._lock;
-    rewrite (handle_pts_to_aux0 r2) (handle_pts_to_aux r2);
-    rewrite (handle_pts_to0 ts) (handle_pts_to ts);
-    return true
-  end else begin
-    R.share handle.state_ptr;
-    rewrite (state_ptr_lock0 handle.state_ptr) (state_ptr_lock handle.state_ptr);
-    Lock.release handle._lock;
-    let p = vpattern_replace (fun p -> R.pts_to handle.state_ptr p _) in
-    rewrite (R.pts_to handle.state_ptr _ _) (R.pts_to handle.state_ptr p state);
-    with_invariant_g
-      #unit
-      #(R.pts_to handle.state_ptr p state)
-      #(fun _ -> exists_ (fun ts -> handle_pts_to ts))
-      #_
-      #(state_ptr_inv handle.state_ptr)
-      handle._inv
-      (fun _ ->
-        rewrite (state_ptr_inv _) (state_ptr_inv0 handle.state_ptr);
-        let _ = gen_elim () in
-        R.gather _ #state handle.state_ptr;
-        rewrite (state_ptr_inv_if _ _) (state_ptr_inv_not_null state);
-        let _ = gen_elim () in
-        R.share state;
-        share_body _;
-        let p' = vpattern_replace (fun p -> R.pts_to handle.state_ptr p _) in
-        R.share handle.state_ptr;
-        rewrite (state_ptr_inv_not_null state) (state_ptr_inv_if state p');
-        rewrite (state_ptr_inv0 handle.state_ptr) (state_ptr_inv handle.state_ptr);
-        let r2 = vpattern_replace (fun r2 -> R.pts_to state _ r2 `star` handle_pts_to_body r2) in
-        let ts = Ghost.reveal r2.tl_state in
-        rewrite (handle_pts_to_aux0 r2) (handle_pts_to_aux r2);
-        rewrite (handle_pts_to0 ts) (handle_pts_to ts);
-        noop ()
-      );
-    return false
-  end
-
-#pop-options
-
-inline_for_extraction
-let acquire_thread_lock
-  (t: state_t)
-  (tid: AT.tid)
-: STT (Ghost.erased AEH.log)
-    (handle_pts_to_body t)
-    (fun entries -> handle_pts_to_body t `star` M.log_of_tid t.tl_state tid entries)
-= rewrite (handle_pts_to_body t) (handle_pts_to_body0 t);
-  let _ = gen_elim () in
-  let l = A.read t.thread_locks (FStar.Int.Cast.uint16_to_uint32 tid) in
-  Lock.acquire (dsnd l <: Lock.lock (thread_lock_vprop t.tl_state tid));
-  let entries : Ghost.erased AEH.log = elim_exists () in
-  rewrite (handle_pts_to_body0 t) (handle_pts_to_body t);
-  return entries
-
-inline_for_extraction
-let release_thread_lock
-  (t: state_t)
-  (tid: AT.tid)
-  (entries: Ghost.erased AEH.log)
-: STT unit
-    (handle_pts_to_body t `star` M.log_of_tid t.tl_state tid entries)
-    (fun _ -> handle_pts_to_body t)
-= rewrite (handle_pts_to_body t) (handle_pts_to_body0 t);
-  let _ = gen_elim () in
-  let l = A.read t.thread_locks (FStar.Int.Cast.uint16_to_uint32 tid) in
-  Lock.release (dsnd l <: Lock.lock (thread_lock_vprop t.tl_state tid));
-  rewrite (handle_pts_to_body0 t) (handle_pts_to_body t)
 
 #push-options "--z3rlimit 32 --query_stats --ifuel 6"
 #restart-solver
@@ -619,139 +104,131 @@ let m_verify_post_failure_eq
        exists_ (fun s -> A.pts_to output full_perm s) `star`
        exists_ (fun entries' -> M.log_of_tid t tid entries')))
 
-let verify_log_some
-               (t0: Ghost.erased state_t)
+let verify_log_some_concl
+  (#opened: _)
                (tid:U16.t)
                (#log_perm:perm)
                (#log_bytes:Ghost.erased AT.bytes)
                (len: U32.t)
-               (input: EXT.extern_ptr U8.t)
+               (input: EXT.extern_ptr)
                (out_len: U32.t)
                (#out_bytes:Ghost.erased AT.bytes)
-               (output: EXT.extern_ptr U8.t)
-  : ST (verify_result len)
-    (handle_pts_to_aux t0 `star` verify_pre log_perm log_bytes input out_bytes output)
+               (output: EXT.extern_ptr)
+               (sq: squash (check_verify_input tid len input out_len output))
+               (input': U.larray U8.t len)
+               (output' : U.larray U8.t out_len)
+               (entries: Ghost.erased AEH.log)
+  (p1 p2: perm)
+  (v: option (v:V.verify_result { V.verify_result_complete len v }))
+: STGhost (Ghost.erased AEH.log) opened
+    (R.pts_to handle.state.state p1 handle.state.tl_state `star` A.pts_to handle.state.thread_locks p2 handle.state.tl_thread_locks `star` M.frozen_logs handle.state.tl_state handle.state.tl_frozen_logs `star` M.verify_post handle.state.tl_state tid entries log_perm log_bytes len input' out_len out_bytes output' v)
+    (fun entries -> verify_post tid log_perm log_bytes len input out_len out_bytes output v `star` M.log_of_tid handle.state.tl_state tid entries)
+    (input' == EXT.gtake input /\ output' == EXT.gtake output)
+    (fun _ -> True)
+= if (Some? v && V.Verify_success? (Some?.v v))
+  then begin
+    let Some (V.Verify_success read wrote) = v in
+    rewrite
+      (M.verify_post _ tid entries log_perm log_bytes len input' out_len out_bytes output' _)
+      (M.core_inv handle.state.tl_state `star`
+        A.pts_to (EXT.gtake input) log_perm log_bytes `star`
+        exists_ (M.verify_post_success_pred handle.state.tl_state tid entries log_bytes out_len out_bytes output' read wrote)
+      );
+    let _ = gen_elim () in
+    rewrite (handle_pts_to_body0 handle.state) (handle_pts_to_body handle.state);
+    let entries' = vpattern_erased (fun entries' -> M.log_of_tid handle.state.tl_state tid (_ `Seq.append` entries')) in
+    let entries_f = vpattern_replace_erased (fun (entries_: AEH.log) -> M.log_of_tid handle.state.tl_state tid entries_) in
+    rewrite (handle_pts_to0 handle.state.tl_state) (handle_pts_to handle.state.tl_state);
+    let out_bytes' = vpattern_replace_erased (A.pts_to output' _) in
+    vpattern_rewrite #_ #_ #output' (fun output -> A.pts_to output _ _) (EXT.gtake output);
+    assert_ (verify_post_some_m_success_body tid log_perm log_bytes len input out_len out_bytes output v () handle.state.tl_state entries read wrote entries' out_bytes' `star` M.log_of_tid  handle.state.tl_state tid entries_f);
+    rewrite
+      (verify_post_some_m_success tid log_perm log_bytes len input out_len out_bytes output v () handle.state.tl_state read wrote)
+      (verify_post_some_m tid log_perm log_bytes len input out_len out_bytes output v handle.state.tl_state);
+    rewrite
+      (verify_post_some tid log_perm log_bytes len input out_len out_bytes output _)
+      (verify_post tid log_perm log_bytes len input out_len out_bytes output v);
+    entries_f
+  end else begin
+    m_verify_post_failure_eq handle.state.tl_state tid entries log_perm log_bytes len input' out_len out_bytes output' v;
+    let _ = gen_elim () in
+    rewrite (handle_pts_to_body0 handle.state) (handle_pts_to_body handle.state);
+    let entries_f = vpattern_replace_erased (fun (entries_: AEH.log) -> M.log_of_tid handle.state.tl_state tid entries_) in
+    rewrite (handle_pts_to0 handle.state.tl_state) (handle_pts_to handle.state.tl_state);
+    vpattern_rewrite #_ #_ #output' (fun output -> A.pts_to output _ _) (EXT.gtake output);
+    rewrite
+      (verify_post_some_m_failure output)
+      (verify_post_some_m tid log_perm log_bytes len input out_len out_bytes output v handle.state.tl_state);
+    vpattern_rewrite #_ #_ #input' (fun input -> A.pts_to input _ _) (EXT.gtake input);
+    rewrite
+      (verify_post_some tid log_perm log_bytes len input out_len out_bytes output _)
+      (verify_post tid log_perm log_bytes len input out_len out_bytes output v);
+    entries_f
+  end
+
+let verify_log_some
+               (tid:U16.t)
+               (#log_perm:perm)
+               (#log_bytes:Ghost.erased AT.bytes)
+               (len: U32.t)
+               (input: EXT.extern_ptr)
+               (out_len: U32.t)
+               (#out_bytes:Ghost.erased AT.bytes)
+               (output: EXT.extern_ptr)
+  : ST (option (v:V.verify_result { V.verify_result_complete len v }))
+    (handle_pts_to_body handle.state `star` verify_pre log_perm log_bytes input out_bytes output)
     (fun res -> verify_post tid log_perm log_bytes len input out_len out_bytes output res)
     (check_verify_input tid len input out_len output)
     (fun _ -> True)
-= rewrite (handle_pts_to_aux t0) (handle_pts_to_aux0 t0);
+=
+  rewrite (handle_pts_to_body handle.state) (handle_pts_to_body0 handle.state);
   let _ = gen_elim () in
-  let r1 = R.read handle.state_ptr in
-  vpattern_rewrite (fun r1 -> R.pts_to handle.state_ptr _ r1 `star` R.pts_to r1 _ _) r1;
-  let r2 = R.read r1 in
-  vpattern_rewrite (fun r2 -> R.pts_to r1 _ r2 `star` handle_pts_to_body r2) r2;
-  let entries = acquire_thread_lock _ tid in
-  rewrite (handle_pts_to_body r2) (handle_pts_to_body0 r2);
+  let pl : thread_lock_t handle.state.tl_state = A.read handle.state.thread_locks (FStar.Int.Cast.uint16_to_uint32 tid) in
+  let l : Lock.lock (thread_lock_vprop handle.state.tl_state tid) = dsnd pl in
+  Lock.acquire l;
   let _ = gen_elim () in
+  let entries = vpattern_replace_erased (fun (entries: AEH.log) -> M.log_of_tid handle.state.tl_state tid entries) in
   let input' = EXT.take input len in
   let output' = EXT.take output out_len in
   vpattern_rewrite (fun a -> A.pts_to a log_perm log_bytes) input';
   vpattern_rewrite (fun a -> A.pts_to a full_perm out_bytes) output';
   let v = M.verify_log _ tid len input' out_len output' in
-  let res = Some v in
-  let t = r2.tl_state in
-  match v returns STT (verify_result len) (R.pts_to handle.state_ptr _ r1 `star` R.pts_to r1 _ r2 `star` R.pts_to r2.state _ _ `star` A.pts_to r2.thread_locks _ _ `star` M.frozen_logs _ _ `star` M.verify_post _ tid entries log_perm log_bytes len input' out_len out_bytes output' v) (fun res -> verify_post tid log_perm log_bytes len input out_len out_bytes output res) with
-  | Some (V.Verify_success read wrote) ->
-    rewrite
-      (M.verify_post _ tid entries log_perm log_bytes len input' out_len out_bytes output' _)
-      (M.core_inv r2.tl_state `star`
-        A.pts_to (EXT.gtake input) log_perm log_bytes `star`
-        exists_ (M.verify_post_success_pred t tid entries log_bytes out_len out_bytes output' read wrote)
-      );
-    let _ = gen_elim () in
-    rewrite (handle_pts_to_body0 r2) (handle_pts_to_body r2);
-    let entries' = vpattern_erased (fun entries' -> M.log_of_tid t tid (_ `Seq.append` entries')) in
-    vpattern_rewrite (fun t -> M.log_of_tid t _ _) r2.tl_state;
-    release_thread_lock _ tid _;
-    rewrite (handle_pts_to_aux0 r2) (handle_pts_to_aux r2);
-    rewrite (handle_pts_to0 t) (handle_pts_to t);
-    let out_bytes' = vpattern_replace_erased (A.pts_to output' _) in
-    vpattern_rewrite #_ #_ #output' (fun output -> A.pts_to output _ _) (EXT.gtake output);
-    assert_ (verify_post_some_m_success_body tid log_perm log_bytes len input out_len out_bytes output v () t entries read wrote entries' out_bytes');
-    rewrite
-      (verify_post_some_m_success tid log_perm log_bytes len input out_len out_bytes output v () t entries read wrote)
-      (verify_post_some_m tid log_perm log_bytes len input out_len out_bytes output v () t entries);
-    rewrite
-      (verify_post_some tid log_perm log_bytes len input out_len out_bytes output v ())
-      (verify_post tid log_perm log_bytes len input out_len out_bytes output res);
-    return res
-  | v ->
-    m_verify_post_failure_eq r2.tl_state tid entries log_perm log_bytes len input' out_len out_bytes output' v;
-    let _ = gen_elim () in
-    rewrite (handle_pts_to_body0 r2) (handle_pts_to_body r2);
-    vpattern_rewrite (fun t -> M.log_of_tid t _ _) r2.tl_state;
-    release_thread_lock _ tid _;
-    rewrite (handle_pts_to_aux0 r2) (handle_pts_to_aux r2);
-    rewrite (handle_pts_to0 t) (handle_pts_to t);
-    vpattern_rewrite #_ #_ #output' (fun output -> A.pts_to output _ _) (EXT.gtake output);
-    rewrite
-      (verify_post_some_m_failure output)
-      (verify_post_some_m tid log_perm log_bytes len input out_len out_bytes output v () t entries);
-    vpattern_rewrite #_ #_ #input' (fun input -> A.pts_to input _ _) (EXT.gtake input);
-    rewrite
-      (verify_post_some tid log_perm log_bytes len input out_len out_bytes output v ())
-      (verify_post tid log_perm log_bytes len input out_len out_bytes output res);
-    return res
+  let _ = verify_log_some_concl tid len input out_len output () input' output' entries _ _ v in
+  Lock.release l;
+  return v
 
 let verify_log
   tid #log_perm #log_bytes len input out_len #out_bytes output
 =
-  if not (check_verify_input tid len input out_len output) returns STT (verify_result len)
-    (verify_pre log_perm log_bytes input out_bytes output)
+  let t = handle.state.tl_state in
+  handle_pts_to_body_intro ();
+  if not (check_verify_input tid len input out_len output) returns STT (option (v:V.verify_result { V.verify_result_complete len v }))
+    (handle_pts_to_body handle.state `star` verify_pre log_perm log_bytes input out_bytes output)
     (fun res -> verify_post tid log_perm log_bytes len input out_len out_bytes output res)
   then begin
     noop ();
-    rewrite (verify_pre log_perm log_bytes input out_bytes output)
+    rewrite (handle_pts_to0 t) (handle_pts_to t);
+    rewrite (verify_post_some_m_failure output) (verify_post_some_m tid log_perm log_bytes len input out_len out_bytes output None t);
+    rewrite (verify_post_some tid log_perm log_bytes len input out_len out_bytes output None)
       (verify_post tid log_perm log_bytes len input out_len out_bytes output None);
     return None
   end else
-  let is_null = handle_is_null () in
-  if is_null
-  then begin
-    noop ();
-    rewrite (handle_is_null_post _) emp;
-    rewrite (verify_pre log_perm log_bytes input out_bytes output)
-      (verify_post tid log_perm log_bytes len input out_len out_bytes output None);
-    return None
-  end else 
   begin
     noop ();
-    rewrite (handle_is_null_post _) (exists_ handle_pts_to_aux);
-    let ts = elim_exists () in
-    verify_log_some ts tid len input out_len output
+    verify_log_some tid len input out_len output
   end
 
 let max_certified_epoch
   ()
 =
-  let is_null = handle_is_null () in
-  if is_null
-  then begin
-    noop ();
-    rewrite (handle_is_null_post _) (max_certified_epoch_post None);
-    return None
-  end else 
-  begin
-    noop ();
-    rewrite (handle_is_null_post _) (exists_ handle_pts_to_aux);
-    let t0 = elim_exists () in
-    rewrite (handle_pts_to_aux t0) (handle_pts_to_aux0 t0);
+    handle_pts_to_body_intro ();
+    rewrite (handle_pts_to_body handle.state) (handle_pts_to_body0 handle.state);
     let _ = gen_elim () in
-    let r1 = R.read handle.state_ptr in
-    vpattern_rewrite (fun r1 -> R.pts_to handle.state_ptr _ r1 `star` R.pts_to r1 _ _) r1;
-    let r2 = R.read r1 in
-    vpattern_rewrite (fun r2 -> R.pts_to r1 _ r2 `star` handle_pts_to_body r2) r2;
-    rewrite (handle_pts_to_body r2) (handle_pts_to_body0 r2);
-    let _ = gen_elim () in
-    let t = r2.tl_state in
-    let r = M.max_certified_epoch r2.state in
+    let t = handle.state.tl_state in
+    let r = M.max_certified_epoch handle.state.state in
     vpattern_rewrite (fun t -> M.read_max_post t _) t;
-    rewrite (handle_pts_to_body0 r2) (handle_pts_to_body r2);
-    rewrite (handle_pts_to_aux0 r2) (handle_pts_to_aux r2);
+    rewrite (handle_pts_to_body0 handle.state) (handle_pts_to_body handle.state);
     rewrite (handle_pts_to0 t) (handle_pts_to t);
-    let res = Some r in
-    rewrite (max_certified_epoch_post_some r) (max_certified_epoch_post res);
-    return res
-  end
+    return r
 
 #pop-options
