steel/Zeta.Steel.SafeMain.fsti
@@ -34,22 +34,13 @@ val share
     (handle_pts_to ts)
     (fun _ -> handle_pts_to ts `star` handle_pts_to ts)
 
-val init (_: unit) : STT bool
-  emp
-  (fun b ->
-    exists_ (fun ts ->
-      handle_pts_to ts // we lost the all_logs ... (Map.const (Some Seq.empty)) post-resource because it is consumed when creating thread locks
-  ))
-
-let verify_result (len: U32.t) = option (option (v:V.verify_result { V.verify_result_complete len v }))
-
 [@__reduce__]
 let verify_pre
     (log_perm:perm)
     (log_bytes: AT.bytes)
-    (input: EXT.extern_ptr U8.t)
+    (input: EXT.extern_ptr)
     (out_bytes: AT.bytes)
-    (output: EXT.extern_ptr U8.t)
+    (output: EXT.extern_ptr)
 : Tot vprop
 =
      A.pts_to (EXT.gtake input) log_perm log_bytes `star`
@@ -58,10 +49,10 @@ let verify_pre
 inline_for_extraction
 let check_verify_input
   (tid: U16.t)
-  (len: U32.t) // { len <> 0ul })
-  (input: EXT.extern_ptr U8.t) // U.larray U8.t len)
+  (len: U32.t)
+  (input: EXT.extern_ptr)
   (out_len: U32.t)
-  (output: EXT.extern_ptr U8.t) // U.larray U8.t out_len)
+  (output: EXT.extern_ptr)
 : Tot bool
 = FStar.Int.Cast.uint16_to_uint32 tid `U32.lt` AT.n_threads &&
   len <> 0ul &&
@@ -73,11 +64,11 @@ let verify_post_some_m_success_body
   (tid:U16.t)
   (log_perm:perm)
   (log_bytes: AT.bytes)
-  (len: U32.t) // { len <> 0ul })
-  (input: EXT.extern_ptr U8.t) // U.larray U8.t len)
+  (len: U32.t)
+  (input: EXT.extern_ptr)
   (out_len: U32.t)
   (out_bytes: AT.bytes)
-  (output: EXT.extern_ptr U8.t) // U.larray U8.t out_len)
+  (output: EXT.extern_ptr)
   (v: option (v:V.verify_result { V.verify_result_complete len v }))
   (sq: squash (check_verify_input tid len input out_len output))
   (t: M.top_level_state)
@@ -104,26 +95,25 @@ let verify_post_some_m_success
   (tid:U16.t)
   (log_perm:perm)
   (log_bytes: AT.bytes)
-  (len: U32.t) // { len <> 0ul })
-  (input: EXT.extern_ptr U8.t) // U.larray U8.t len)
+  (len: U32.t)
+  (input: EXT.extern_ptr)
   (out_len: U32.t)
   (out_bytes: AT.bytes)
-  (output: EXT.extern_ptr U8.t) // U.larray U8.t out_len)
+  (output: EXT.extern_ptr)
   (v: option (v:V.verify_result { V.verify_result_complete len v }))
   (sq: squash (check_verify_input tid len input out_len output))
   (t: M.top_level_state)
-  (entries: _)
   (read:U32.t)
   (wrote:U32.t)
 : Tot vprop
 =
-       exists_ (fun entries' -> exists_ (fun out_bytes' ->
+       exists_ (fun entries -> exists_ (fun entries' -> exists_ (fun out_bytes' ->
          verify_post_some_m_success_body tid log_perm log_bytes len input out_len out_bytes output v sq t entries read wrote entries' out_bytes'
-       ))
+       )))
 
 [@@__reduce__]
 let verify_post_some_m_failure
-  (output: EXT.extern_ptr U8.t) // U.larray U8.t out_len)
+  (output: EXT.extern_ptr)
 : Tot vprop
 = exists_ (fun s -> A.pts_to (EXT.gtake output) full_perm s)
 
@@ -131,19 +121,21 @@ let verify_post_some_m
   (tid:U16.t)
   (log_perm:perm)
   (log_bytes: AT.bytes)
-  (len: U32.t) // { len <> 0ul })
-  (input: EXT.extern_ptr U8.t) // U.larray U8.t len)
+  (len: U32.t)
+  (input: EXT.extern_ptr)
   (out_len: U32.t)
   (out_bytes: AT.bytes)
-  (output: EXT.extern_ptr U8.t) // U.larray U8.t out_len)
+  (output: EXT.extern_ptr)
   (v: option (v:V.verify_result { V.verify_result_complete len v }))
-  (sq: squash (check_verify_input tid len input out_len output))
   (t: M.top_level_state)
-  (entries: _)
 : Tot vprop
 = match v with
   | Some (V.Verify_success read wrote) ->
-    verify_post_some_m_success tid log_perm log_bytes len input out_len out_bytes output v sq t entries read wrote
+    if check_verify_input tid len input out_len output
+    then
+      verify_post_some_m_success tid log_perm log_bytes len input out_len out_bytes output v () t read wrote
+    else
+      pure False
   | _ -> verify_post_some_m_failure output 
 
 [@@__reduce__]
@@ -151,69 +143,51 @@ let verify_post_some
   (tid:U16.t)
   (log_perm:perm)
   (log_bytes: AT.bytes)
-  (len: U32.t) // { len <> 0ul })
-  (input: EXT.extern_ptr U8.t) // U.larray U8.t len)
+  (len: U32.t)
+  (input: EXT.extern_ptr)
   (out_len: U32.t)
   (out_bytes: AT.bytes)
-  (output: EXT.extern_ptr U8.t) // U.larray U8.t out_len)
+  (output: EXT.extern_ptr)
   (v: option (v:V.verify_result { V.verify_result_complete len v }))
-  (sq: squash (check_verify_input tid len input out_len output))
 : Tot vprop
 = 
-    exists_ (fun t -> exists_ (fun entries ->
+    exists_ (fun t ->
       handle_pts_to t `star`
       A.pts_to (EXT.gtake input) log_perm log_bytes `star`
-      verify_post_some_m tid log_perm log_bytes len input out_len out_bytes output v sq t entries
-    ))
+      verify_post_some_m tid log_perm log_bytes len input out_len out_bytes output v t
+    )
 
 let verify_post
   (tid:U16.t)
   (log_perm:perm)
   (log_bytes: AT.bytes)
-  (len: U32.t) // { len <> 0ul })
-  (input: EXT.extern_ptr U8.t) // U.larray U8.t len)
+  (len: U32.t)
+  (input: EXT.extern_ptr)
   (out_len: U32.t)
   (out_bytes: AT.bytes)
-  (output: EXT.extern_ptr U8.t) // U.larray U8.t out_len)
-  (res: verify_result len)
+  (output: EXT.extern_ptr)
+  (res: option (v:V.verify_result { V.verify_result_complete len v }))
 : Tot vprop
-= match res with
-  | None -> verify_pre log_perm log_bytes input out_bytes output
-  | Some v ->
-    if check_verify_input tid len input out_len output
-    then verify_post_some tid log_perm log_bytes len input out_len out_bytes output v ()
-    else pure False
+= verify_post_some tid log_perm log_bytes len input out_len out_bytes output res
 
 val verify_log
                (tid:U16.t)
                (#log_perm:perm)
                (#log_bytes:Ghost.erased AT.bytes)
                (len: U32.t)
-               (input: EXT.extern_ptr U8.t)
+               (input: EXT.extern_ptr)
                (out_len: U32.t)
                (#out_bytes:Ghost.erased AT.bytes)
-               (output: EXT.extern_ptr U8.t)
-  : STT (verify_result len)
+               (output: EXT.extern_ptr)
+  : STT (option (v:V.verify_result { V.verify_result_complete len v }))
     (verify_pre log_perm log_bytes input out_bytes output)
     (fun res -> verify_post tid log_perm log_bytes len input out_len out_bytes output res)
 
-[@@__reduce__]
-let max_certified_epoch_post_some
-  (res: AEH.max_certified_epoch_result)
-: Tot vprop
-=
-  exists_ (fun t -> handle_pts_to t `star`
-    M.read_max_post t res)
-
-let max_certified_epoch_post
-  (res: option AEH.max_certified_epoch_result)
-: Tot vprop
-= match res with
-  | None -> emp
-  | Some res -> max_certified_epoch_post_some res
-
 val max_certified_epoch
                         (_: unit)
-  : STT (option AEH.max_certified_epoch_result)
+  : STT AEH.max_certified_epoch_result
         emp
-        (fun res -> max_certified_epoch_post res)
+        (fun res -> exists_ (fun t ->
+          handle_pts_to t `star`
+          M.read_max_post t res
+        ))
