steel/Zeta.Steel.SafeMain.Handle.fst
@@ -1,0 +1,200 @@
+module Zeta.Steel.SafeMain.Handle
+
+module M = Zeta.Steel.Main
+module AEH = Zeta.Steel.AggregateEpochHashes
+module AT = Zeta.Steel.ApplicationTypes
+module U16 = FStar.UInt16
+module U32 = FStar.UInt32
+
+module Lock = Steel.ST.SpinLock
+module R = Steel.ST.Reference
+module A = Steel.ST.Array
+
+open Steel.ST.GenElim
+
+// TODO: use FStarLang/FStar#2349 to nest structs and take pointers to fields. However, we need support for atomic accesses for such references, at least for the top-level cases (so far we don't need atomic field accesses here yet)
+
+[@@__reduce__]
+let thread_lock_vprop
+  (tl_state: M.top_level_state)
+  (tid: AT.tid)
+: Tot vprop
+= exists_ (fun (entries: AEH.log) -> M.log_of_tid tl_state tid entries)
+
+let thread_lock_t
+  (tl_state: M.top_level_state)
+: Tot Type
+= (tid: Ghost.erased AT.tid & Lock.lock (thread_lock_vprop tl_state tid))
+
+let thread_state_prop
+  (#tl_state: M.top_level_state)
+  (a: Seq.seq (thread_lock_t tl_state))
+: Tot prop
+= forall (i: nat { i < Seq.length a }) . {:pattern (Seq.index a i)} U16.v (dfst (Seq.index a i)) == i
+
+noeq
+type state_t = {
+  state: R.ref M.top_level_state;
+  tl_state: Ghost.erased M.top_level_state;
+  thread_locks: A.array (thread_lock_t tl_state);
+  tl_thread_locks: Ghost.erased (Seq.seq (thread_lock_t tl_state));
+  tl_frozen_logs: Ghost.erased M.tid_log_map;
+  tl_prf: squash (thread_state_prop tl_thread_locks /\ Seq.length tl_thread_locks == U32.v AT.n_threads);
+}
+
+[@@__reduce__]
+let handle_pts_to_body0
+  (r2: state_t)
+: Tot vprop
+= exists_ (fun p3 -> exists_ (fun p4 ->
+    R.pts_to r2.state p3 r2.tl_state `star`
+    A.pts_to r2.thread_locks p4 r2.tl_thread_locks `star`
+    M.core_inv r2.tl_state `star`
+    M.frozen_logs r2.tl_state r2.tl_frozen_logs
+  ))
+
+let handle_pts_to_body
+  (r2: state_t)
+: Tot vprop
+= handle_pts_to_body0 r2
+
+let gather_body
+  (#opened: _)
+  (r2: state_t)
+: STGhostT unit opened
+    (handle_pts_to_body r2 `star` handle_pts_to_body r2)
+    (fun _ -> handle_pts_to_body r2)
+= rewrite (handle_pts_to_body r2) (handle_pts_to_body0 r2);
+  let _ = gen_elim () in
+  let ps = vpattern_replace (fun ps -> R.pts_to r2.state ps _) in
+  let pa = vpattern_replace (fun pa -> A.pts_to r2.thread_locks pa _) in
+  rewrite (handle_pts_to_body r2) (handle_pts_to_body0 r2);
+  let _ = gen_elim () in
+  A.gather r2.thread_locks pa _;
+  R.gather ps r2.state;
+  M.core_inv_gather _;
+  M.frozen_logs_gather _ _;
+  rewrite (handle_pts_to_body0 r2) (handle_pts_to_body r2)
+
+let share_body
+  (#opened: _)
+  (r2: state_t)
+: STGhostT unit opened
+    (handle_pts_to_body r2)
+    (fun _ -> handle_pts_to_body r2 `star` handle_pts_to_body r2)
+= rewrite (handle_pts_to_body r2) (handle_pts_to_body0 r2);
+  let _ = gen_elim () in
+  let pa = vpattern_replace (fun pa -> A.pts_to r2.thread_locks pa _) in
+  A.share r2.thread_locks pa (half_perm pa) (half_perm pa);
+  R.share r2.state;
+  M.core_inv_share _;
+  M.frozen_logs_share _ _;
+  rewrite (handle_pts_to_body0 r2) (handle_pts_to_body r2);
+  noop ();
+  rewrite (handle_pts_to_body0 r2) (handle_pts_to_body r2)
+
+let seq_lemma_index_upd
+  (#a:Type)
+  (s:Seq.seq a)
+  (n:nat{n < Seq.length s})
+  (v:a)
+: Lemma
+  (requires True)
+  (ensures (forall i . Seq.index (Seq.upd s n v) i == (if i = n then v else Seq.index s i)))
+= ()
+
+// TODO: replace this function with a Steel.ST.Loops.while_loop
+let rec init_thread_locks_loop
+  (tl_state: Ghost.erased M.top_level_state)
+  (tl_logs: Ghost.erased M.tid_log_map)
+  (tl: A.array (thread_lock_t tl_state))
+  (a0: Ghost.erased (Seq.seq (thread_lock_t tl_state)))
+  (tid: U16.t)
+: ST unit
+    (M.all_logs tl_state tl_logs `star` A.pts_to tl full_perm a0)
+    (fun _ ->
+      exists_ (fun l' -> M.frozen_logs tl_state l') `star`
+      exists_ (fun a ->
+      A.pts_to tl full_perm a `star`
+      pure (thread_state_prop a /\ Seq.length a == U32.v AT.n_threads)
+    ))
+    (A.length tl == U32.v AT.n_threads /\
+      Seq.length (Ghost.reveal a0) == U32.v AT.n_threads /\
+      U16.v tid <= U32.v AT.n_threads /\
+      (forall (i: nat) . i < U16.v tid ==> U16.v (Ghost.reveal (dfst (Seq.index (Ghost.reveal a0) i))) == i) /\
+      (forall (i: AT.tid) . U16.v i >= U16.v tid ==> Some? (Map.sel tl_logs i))
+    )
+    (fun _ -> True)
+= let tid32 = FStar.Int.Cast.uint16_to_uint32 tid in
+  if tid32 = AT.n_threads
+  then begin
+    M.freeze_all_logs _ _;
+    return ()
+  end
+  else begin
+    M.all_logs_log_of_tid _ _ tid ();
+    let l = Lock.new_lock (thread_lock_vprop tl_state tid) in
+    let t : thread_lock_t tl_state = (| Ghost.hide tid, l |) in
+    A.write tl tid32 t;
+    Seq.lemma_len_upd (U32.v tid32) t a0;
+    seq_lemma_index_upd a0 (U32.v tid32) t;
+    init_thread_locks_loop tl_state _ tl _ (tid `U16.add` 1us)
+  end
+
+let init_thread_locks
+  (tl_state: Ghost.erased M.top_level_state)
+  (tl_logs: Ghost.erased M.tid_log_map)
+: ST (A.array (thread_lock_t tl_state))
+    (M.all_logs tl_state tl_logs)
+    (fun tl ->
+      exists_ (fun l' -> M.frozen_logs tl_state l') `star`
+      exists_ (fun a ->
+        A.pts_to tl full_perm a `star`
+        pure (thread_state_prop a /\ Seq.length a == U32.v AT.n_threads)
+    ))
+    (forall (i: AT.tid) . Some? (Map.sel tl_logs i))
+    (fun _ -> True)
+= M.all_logs_log_of_tid _ _ 0us ();
+  let l0 = Lock.new_lock (thread_lock_vprop tl_state 0us) in
+  let tl0: thread_lock_t tl_state = (| Ghost.hide 0us, l0 |) in
+  let tl = A.alloc tl0 AT.n_threads in
+  Seq.lemma_create_len (U32.v AT.n_threads) tl0;
+  Seq.lemma_index_create (U32.v AT.n_threads) tl0 0;
+  init_thread_locks_loop _ _ tl _ 1us;
+  return tl
+
+noeq
+type handle_t = {
+  state: state_t;
+  _inv: inv (handle_pts_to_body state);
+}
+
+let handle: handle_t =
+  begin
+    let r2_state = M.init () in
+    let ts = elim_exists () in
+    let tl = init_thread_locks ts _ in
+    let _ = gen_elim () in
+    let tl_f = vpattern_replace_erased (M.frozen_logs ts) in
+    let tl_a = vpattern_replace_erased (A.pts_to tl _) in
+    [@@inline_let]
+    let r2 : state_t = ({
+      state = r2_state;
+      tl_state = ts;
+      thread_locks = tl;
+      tl_thread_locks = tl_a;
+      tl_frozen_logs = tl_f;
+      tl_prf = ();
+    })
+    in
+    rewrite (R.pts_to r2_state full_perm _) (R.pts_to r2.state full_perm r2.tl_state);
+    rewrite (A.pts_to _ _ _) (A.pts_to r2.thread_locks full_perm r2.tl_thread_locks);
+    rewrite (M.frozen_logs _ _) (M.frozen_logs r2.tl_state r2.tl_frozen_logs);
+    vpattern_rewrite M.core_inv (Ghost.reveal r2.tl_state);
+    rewrite (handle_pts_to_body0 r2) (handle_pts_to_body r2);
+    let i = new_invariant (handle_pts_to_body r2) in
+    return ({
+      state = r2;
+      _inv = i;
+    })
+  end <: STT handle_t emp (fun _ -> emp)
